Replace IteratorInv with StackInv

correctness/RegexCorrectness/Backtracker/Path.lean
@@ -1,8 +1,10 @@
+import RegexCorrectness.Data.BoundedIterator
 import RegexCorrectness.NFA.Semantics.Path
 
 set_option autoImplicit false
 
 open String (Iterator)
+open Regex.Data (BoundedIterator)
 
 namespace Regex.Backtracker
 
@@ -32,6 +34,12 @@ theorem toString_eq {nfa : NFA} {wf : nfa.WellFormed} {it it' i update} (path : 
   | init => rfl
   | more prev step equpdate ih => rw [step.toString_eq, ih]
 
+theorem le_pos {nfa : NFA} {wf : nfa.WellFormed} {it it' i update} (path : Path nfa wf it it' i update) :
+  it.pos ≤ it'.pos := by
+  induction path with
+  | init _ => exact Nat.le_refl _
+  | more _ step _ ih => exact Nat.le_trans ih step.le_pos
+
 theorem eq_or_nfaPath {nfa : NFA} {wf : nfa.WellFormed} {it it' i update} (path : Path nfa wf it it' i update) :
   (it' = it ∧ i.val = nfa.start ∧ update = []) ∨
   nfa.Path 0 nfa.start it i it' update := by
@@ -49,6 +57,33 @@ theorem eq_or_nfaPath {nfa : NFA} {wf : nfa.WellFormed} {it it' i update} (path 
 theorem nfaPath_of_ne {nfa : NFA} {wf : nfa.WellFormed} {it it' i update} (path : Path nfa wf it it' i update) (ne : i.val ≠ nfa.start) :
   nfa.Path 0 nfa.start it i it' update := by
   simpa [ne] using eq_or_nfaPath path
+
+def bit' {nfa : NFA} {wf : nfa.WellFormed} {startIdx maxIdx : Nat} {bit : BoundedIterator startIdx maxIdx} {it' i update}
+  (path : Path nfa wf bit.it it' i update) : BoundedIterator startIdx maxIdx :=
+  have gem : startIdx ≤ it'.pos.byteIdx := Nat.le_trans bit.ge path.le_pos
+  have eqm : maxIdx = it'.toString.endPos.byteIdx := path.toString_eq ▸ bit.eq
+  have lem : it'.pos.byteIdx ≤ maxIdx := eqm ▸ path.validR.le_endPos
+  ⟨it', gem, lem, eqm⟩
+
+theorem isNextNOf {nfa : NFA} {wf : nfa.WellFormed} {startIdx maxIdx : Nat} {bit bit' : BoundedIterator startIdx maxIdx} {it' i update}
+  (eqit' : bit'.it = it') (path : Path nfa wf bit.it it' i update) :
+  bit'.IsNextNOf bit := by
+  induction path generalizing bit' with
+  | init v =>
+    have eq : bit' = bit := by
+      simp [BoundedIterator.ext_iff, eqit']
+    exact ⟨0, by simp [eq, BoundedIterator.nextn]⟩
+  | @more i j itm it' update₁ update₂ update₃ prev step equpdate ih =>
+    have isNextN := @ih prev.bit' rfl
+    match step.it_eq_or_next with
+    | .inl eq =>
+      have eq' : bit' = prev.bit' := by
+        simp [BoundedIterator.ext_iff, eqit', eq, Path.bit']
+      simpa [eq'] using isNextN
+    | .inr ⟨hnext, eq⟩ =>
+      have eq' : bit' = prev.bit'.next hnext := by
+        simp [BoundedIterator.ext_iff, eqit', eq, Path.bit', BoundedIterator.next, Iterator.next'_eq_next]
+      simpa [eq'] using isNextN.next hnext
 
 end Path
 
